Added copy and ocaml blit functions

lib/arr.fst
@@ -78,3 +78,85 @@ let swap x i j =
   let h1 = get () in
   let s1 = sel h1 x in
   cut (b2t(equal h1 (Heap.upd h0 x s1)))
+
+(* Helper functions for stateful array manipulation *)
+val array_copy_aux:
+  s:array int -> cpy:array int -> ctr:nat ->
+  ST unit
+     (requires (fun h -> (contains h s /\ contains h cpy /\ s <> cpy)
+			 /\ (Seq.length (sel h cpy) = Seq.length (sel h s))
+			 /\ (ctr <= Seq.length (sel h cpy))
+			 /\ (forall (i:nat). i < ctr ==> Seq.index (sel h s) i = Seq.index (sel h cpy) i)))
+     (ensures (fun h0 u h1 -> (contains h1 s /\ contains h1 cpy /\ s <> cpy )
+			      /\ (modifies !{cpy} h0 h1)
+			      /\ (Seq.Eq (sel h1 cpy) (sel h1 s))))
+let rec array_copy_aux s cpy ctr =
+  match Array.length cpy - ctr with
+  | 0 -> ()
+  | _ -> Array.upd cpy ctr (Array.index s ctr);
+	 array_copy_aux s cpy (ctr+1)
+
+val array_copy: 
+	 s:array int -> 
+	 ST (array int)
+	    (requires (fun h -> contains h s))
+	    (ensures (fun h0 r h1 -> (modifies !{} h0 h1)
+				     /\ not(contains h0 r)
+				     /\ (contains h1 r)
+				     /\ (Seq.Eq (sel h1 r) (sel h0 s))))
+let array_copy s =
+  let cpy = Array.create (Array.length s) 0 in
+  array_copy_aux s cpy 0;
+  cpy
+
+val array_blit_aux:
+  s:array int -> s_idx:nat -> t:array int -> t_idx:nat -> len:nat -> ctr:nat ->
+  ST unit
+     (requires (fun h -> 
+		(contains h s /\ contains h t /\ s <> t)
+		/\ (Seq.length (sel h s) >= s_idx + len)
+		/\ (Seq.length (sel h t) >= t_idx + len)
+		/\ (ctr <= len)
+		/\ (forall (i:nat). 
+		    i < ctr ==> Seq.index (sel h s) (s_idx+i) = Seq.index (sel h t) (t_idx+i))))
+     (ensures (fun h0 u h1 -> 
+	       (contains h1 s /\ contains h1 t /\ s <> t )
+	       /\ (modifies !{t} h0 h1)
+	       /\ (Seq.length (sel h1 s) >= s_idx + len)
+	       /\ (Seq.length (sel h1 t) >= t_idx + len)
+	       /\ (Seq.length (sel h0 s) = Seq.length (sel h1 s))
+	       /\ (Seq.length (sel h0 t) = Seq.length (sel h1 t))
+	       /\ (forall (i:nat). 
+		   i < len ==> Seq.index (sel h1 s) (s_idx+i) = Seq.index (sel h1 t) (t_idx+i))
+	       /\ (forall (i:nat).
+		   (i < Seq.length (sel h1 t) /\ (i < t_idx \/ i >= t_idx + len)) ==> 
+		     Seq.index (sel h1 t) i = Seq.index (sel h0 t) i) ))
+let rec array_blit_aux s s_idx t t_idx len ctr =
+  match len - ctr with
+  | 0 -> ()
+  | _ -> Array.upd t (t_idx + ctr) (Array.index s (s_idx + ctr));
+	 array_blit_aux s s_idx t t_idx len (ctr+1)
+
+val array_blit:
+  s:array int -> s_idx:nat -> t:array int -> t_idx:nat -> len:nat ->
+  ST unit
+     (requires (fun h -> 
+		(contains h s) 
+		/\ (contains h t)
+		/\ (s <> t)
+		/\ (Seq.length (sel h s) >= s_idx + len)
+		/\ (Seq.length (sel h t) >= t_idx + len)))
+     (ensures (fun h0 u h1 -> 
+	       (contains h1 s /\ contains h1 t /\ s <> t )
+	       /\ (Seq.length (sel h1 s) >= s_idx + len)
+	       /\ (Seq.length (sel h1 t) >= t_idx + len)
+	       /\ (Seq.length (sel h0 s) = Seq.length (sel h1 s))
+	       /\ (Seq.length (sel h0 t) = Seq.length (sel h1 t))
+	       /\ (modifies !{t} h0 h1)
+	       /\ (forall (i:nat). 
+		   i < len ==> Seq.index (sel h1 s) (s_idx+i) = Seq.index (sel h1 t) (t_idx+i))
+	       /\ (forall (i:nat).
+		   (i < Seq.length (sel h1 t) /\ (i < t_idx \/ i >= t_idx + len)) ==> 
+		     (Seq.index (sel h1 t) i = Seq.index (sel h0 t) i)) ))
+let rec array_blit s s_idx t t_idx len =
+  array_blit_aux s s_idx t t_idx len 0
